fix doc in monad.v and hiearchy.v, update README, doc in mmt_sect5.v and parametricity.v, fix doc in fail_monad.v, fix doc in state_monad.v merge smallstep.v files, fix doc in proba_monad.v, fix doc of monad_model.v, rename files in impredicative_set

smallstep.v
@@ -1,15 +1,36 @@
 Require Import Eqdep JMeq List ssreflect.
 Import ListNotations.
-From mathcomp Require Import ssrnat.
+From mathcomp Require Import ssreflect ssrfun ssrbool eqtype ssrnat seq.
+Require Import hierarchy monad state_monad trace_monad monad_model.
 
 (******************************************************************************)
-(* A small-step semantics for an imperative language with a primitive to      *)
-(* record execution trace.                                                    *)
+(*              Application of monadTrace to program semantics                *)
+(*                                                                            *)
+(* Inductive program, Inductive continuation:                                 *)
+(*   Syntax for an imperative language with a primitive to record execution   *)
+(*   trace                                                                    *)
+(* Section OperationalSemantics, Inductive step:                              *)
+(*   A small-step semantics                                                   *)
+(* DenotationalSemantics:                                                     *)
+(*   Denotation given in terms of the state/trace monad                       *)
+(* Section semantics_equivalence:                                             *)
+(*.  Prove that the small-step semantics is equivalent to the denotation      *)
+(* nonce, nonce_twice, countdown, etc.                                        *)
+(*   Examples of programs using traces and their small-step and denotational  *)
+(* semantics.                                                                 *)
+(*                                                                            *)
+(* reference:                                                                *)
+(* - R. Affeldt, D. Nowak, T. Saikawa, A Hierarchy of Monadic Effects for     *)
+(* Program Verification using Equational Reasoning, MPC 2019                  *)
 (******************************************************************************)
 
 Set Universe Polymorphism.
 Unset Universe Minimization ToSet.
 Set Polymorphic Inductive Cumulativity.
+
+Set Implicit Arguments.
+Unset Strict Implicit.
+Unset Printing Implicit Defensive.
 
 Set Bullet Behavior "Strict Subproofs".
 
@@ -167,7 +188,7 @@ induction Hss1 as [
   split; [ | split ].
   + exact Hss2.
   + apply ss_refl.
-  + rewrite app_nil_r; reflexivity.
+  + rewrite cats0; reflexivity.
 - intros l2 sk2 Hss2.
   inversion Hss2 as [
     sk1' Hsk1 Hl2 Hsk2
@@ -178,15 +199,15 @@ induction Hss1 as [
     do 3 eexists.
     split; [ apply ss_refl | ].
     split; [ eapply ss_step_None; eassumption | ].
-    rewrite app_nil_r; reflexivity.
+    rewrite cats0; reflexivity.
   + subst sk1' l2' sk2'''.
-    specialize (step_deterministic _ _ _ _ _ Hstep1 Hstep2).
+    specialize (step_deterministic Hstep1 Hstep2).
     intros [ [] Heq2].
     subst sk2''.
     apply IH.
     exact Hss2'.
   + subst sk1' l2 sk2'''.
-    specialize (step_deterministic _ _ _ _ _ Hstep1 Hstep2).
+    specialize (step_deterministic Hstep1 Hstep2).
     intros [ [=] ?].
 - intros l2 sk2 Hss2.
   inversion Hss2 as [
@@ -198,12 +219,12 @@ induction Hss1 as [
     do 3 eexists.
     split; [ apply ss_refl | ].
     split; [ eapply ss_step_Some; eassumption | ].
-    rewrite app_nil_r; reflexivity.
+    rewrite cats0; reflexivity.
   + subst sk1' l2' sk2'''.
-    specialize (step_deterministic _ _ _ _ _ Hstep1 Hstep2).
+    specialize (step_deterministic Hstep1 Hstep2).
     intros [ [=] ?].
   + subst sk1' l2 sk2'''.
-    specialize (step_deterministic _ _ _ _ _ Hstep1 Hstep2).
+    specialize (step_deterministic Hstep1 Hstep2).
     intros [ [= Heq1] Heq2].
     subst t2 sk2''.
     apply IH in Hss2'.
@@ -220,14 +241,14 @@ Lemma step_star_deterministic ski l1 l2 s1 s2 A1 A2 a1 a2 :
   l1 = l2 /\ s1 = s2 /\ A1 = A2 /\ JMeq a1 a2.
 Proof.
 intros Hss1 Hss2.
-specialize (step_star_confluent _ _ _ _ _ Hss1 Hss2).
+specialize (step_star_confluent Hss1 Hss2).
 intros (l1' & l2' & skf & Hss1' & Hss2' & Heq).
 apply step_star_stop_inv in Hss1'.
 apply step_star_stop_inv in Hss2'.
 destruct Hss1' as [ Heq11 Heq12 ].
 destruct Hss2' as [ Heq21 Heq22 ].
 subst l1' l2' skf .
-do 2 rewrite app_nil_r in Heq.
+do 2 rewrite cats0 in Heq.
 injection Heq22; clear Heq22; intros; subst.
 match goal with
 | H : existT _ _ _ = existT _ _ _ |- _ => apply inj_pair2 in H
@@ -358,3 +379,535 @@ Arguments step_star {_ _} _ _ _.
 Arguments run_s {_ _ _} _ _ _.
 Arguments run_s_n {_ _} _ {_} _ _ _.
 Arguments run_ss {_ _ _} _ _.
+
+Local Open Scope monae_scope.
+
+Section DenotationalSemantics.
+
+Variables S T : Type.
+Variable M : stateTraceMonad S T.
+
+Fixpoint denote {A} (p : program A) : M A :=
+  match p with
+  | p_ret _ v => Ret v
+  | p_bind _ _ m f => denote m >>= (denote \o f)
+  | p_cond _ b p1 p2 => if b then denote p1 else denote p2
+  | p_repeat n p => (fix loop m : M unit :=
+    if m is m'.+1 then denote p >> loop m' else Ret tt) n
+  | p_while fuel c p => (fix loop m : M unit :=
+    if m is m'.+1 then
+      (stGet >>= (fun s =>
+      if c s then denote p >> loop m' else Ret tt))
+    else Ret tt) fuel
+  | p_get => stGet
+  | p_put s' => stPut s'
+  | p_mark t => stMark t
+  end.
+
+Notation "'Repeat' n {{ p }}" := (
+  (fix loop (m : nat) : MonadStateTrace.m M unit :=
+   match m with
+   | 0 => Ret tt
+   | m'.+1 => denote p >> loop m'
+   end) n) (at level 200).
+
+Notation "'While' fuel @ c {{ p }}" := (
+  (fix loop (m : nat) : MonadStateTrace.m M unit :=
+   match m with
+   | 0 => Ret tt
+   | m'.+1 =>
+     stGet >>= (fun s =>
+     if c s then denote p >> loop m' else Ret tt)
+   end) fuel) (at level 200).
+
+Fixpoint denote_continuation (k : continuation) : M (@continuation T S) :=
+  match k with
+  | stop A a => Ret (stop A a)
+  | p `; f => denote p >>= (denote_continuation \o f)
+  end.
+
+Definition stateTrace_sub A (m : M A) : Type :=
+  { p | denote p = m }.
+
+Definition continuation_sub (m : M continuation) : Type :=
+  {k | denote_continuation k = m }.
+
+End DenotationalSemantics.
+
+Arguments denote {S} {T} M A.
+Arguments denote_continuation {S} {T} M.
+
+Section semantics_equivalence.
+
+Variables S T : Type.
+Variable M : stateTraceRunMonad S T.
+
+Lemma denote_prefix_preserved A (m : M A) :
+  stateTrace_sub m -> forall s s' l1 l a,
+  Run m (s, l1) = (a, (s', l)) ->
+  exists l2, l = l1 ++ l2.
+Proof.
+case=> p <-{m}.
+induction p as [ A a | A B p IHp g IHg | A b p1 IHp1 p2 IHp2 |
+  n p IHp | fuel c p IHp | | s0 | t ]; cbn;
+ intros s s' l1 l a' Heq.
+- exists [].
+  rewrite cats0.
+  by move: Heq; rewrite runret => -[].
+- rewrite runbind in Heq.
+  case_eq (Run (denote M _ p) (s, l1)).
+  intros a (s0, l0) Hp.
+  rewrite Hp in Heq.
+  move/IHp : Hp => [l2 Hp].
+  move/IHg : Heq => [l2' Heq].
+  exists (l2 ++ l2').
+  by rewrite Heq Hp catA.
+- destruct b; [ eapply IHp1 | eapply IHp2 ]; exact Heq.
+- revert s l1 Heq.
+  induction n as [ | n' IH ]; intros s l1 Heq.
+  + exists [].
+    rewrite cats0.
+    by move: Heq; rewrite runret => -[].
+  + rewrite runbind in Heq.
+    case_eq (Run (denote M _ p) (s, l1)).
+    intros a (s0, l0) Hp.
+    move: (IHp _ _ _ _ _ Hp) => [l2 ?].
+    subst l0.
+    rewrite Hp in Heq.
+    move: (IH _ _ Heq) => [l3 ?].
+    exists (l2 ++ l3).
+    by rewrite catA.
+- revert s l1 Heq.
+  induction fuel as [ | fuel' IH ]; intros s l1 Heq.
+  + exists [].
+    rewrite cats0.
+    by move: Heq; rewrite runret => -[].
+  + rewrite runbind runstget in Heq.
+    destruct (c (s, l1).1).
+    * rewrite runbind in Heq.
+      case_eq (Run (denote M _ p) (s, l1)).
+      intros a (s0, l0) Hp.
+      move: (IHp _ _ _ _ _ Hp) => [l2 ?].
+      subst l0.
+      rewrite Hp in Heq.
+      move: (IH _ _ Heq) => [l3 ?].
+      exists (l2 ++ l3).
+      by rewrite catA.
+    * exists [].
+      rewrite cats0.
+      by move: Heq; rewrite runret => -[].
+- exists [].
+  rewrite cats0.
+  by move: Heq; rewrite runstget => -[].
+- exists [].
+  rewrite cats0.
+  by move: Heq; rewrite runstput => -[].
+- exists [t].
+  by move: Heq; rewrite runstmark -cats1 => -[].
+Qed.
+
+Lemma denote_prefix_independent A (m : M A) :
+  stateTrace_sub m -> forall s l1 l2,
+  Run m (s, l1 ++ l2) =
+  let res := Run m (s, l2) in
+  (res.1, (res.2.1, l1 ++ res.2.2)).
+Proof.
+intros [ p Hp ] s l1 l2.
+subst m.
+elim: p s l1 l2 => /= {A} [A a|A B p1 IH1 p2 IH2|A b p1 IH1 p2 IH2|
+  n p IHp|fuel c p IHp||s'|t] s l1 l2.
+- by rewrite !runret.
+- rewrite [in LHS]runbind [in LHS]IH1.
+  rewrite [in RHS]runbind.
+  case: (Run (denote M _ p1) (s, l2)) => a' [s' l'] /=.
+  by rewrite IH2.
+- by case: ifPn => _; [rewrite IH1|rewrite IH2].
+- revert s l2.
+  induction n as [ | n' IH ]; intros s l2.
+  + by rewrite !runret.
+  + do 2 rewrite runbind.
+    rewrite IHp.
+    clear IHp.
+    case_eq (Run (denote M _ p) (s, l2)).
+    intros a (s0, l0) Hp.
+    exact: IH.
+- revert s l2.
+  induction fuel as [ | fuel' IH ]; intros s l2.
+  + by rewrite !runret.
+  + do 2 rewrite runbind runstget.
+    cbn.
+    destruct (c s).
+    * do 2 rewrite runbind.
+      rewrite IHp.
+      clear IHp.
+      case_eq (Run (denote M _ p) (s, l2)).
+      intros a (s0, l0) Hp.
+      exact: IH.
+    * by rewrite !runret.
+- by rewrite !runstget.
+- by rewrite !runstput.
+- by rewrite !runstmark rcons_cat.
+Qed.
+
+Lemma denote_continuation_prefix_independent (m : M _) :
+  continuation_sub m -> forall s l1 l2,
+  Run m (s, l1 ++ l2) =
+  let res := Run m (s, l2) in
+  (res.1, (res.2.1, l1 ++ res.2.2)).
+Proof.
+intros [ k Hk ].
+subst m.
+elim: k => // [A a s l1 l2|A p k IH s l1 l2].
+by rewrite !runret.
+rewrite /= !runbind.
+rewrite denote_prefix_independent /=; [ | now exists p ].
+destruct (Run (denote M _ p) (s, l2)) as [ a (s', l) ].
+by rewrite IH.
+Qed.
+
+Lemma step_None_correct s s' k k' l :
+  step (s, k) None (s', k') ->
+  Run (denote_continuation M k) (s, l) = Run (denote_continuation M k') (s', l).
+Proof.
+intro Hstep.
+remember (s, k) as sk eqn: Heq.
+remember None as o eqn: Heqo.
+remember (s', k') as sk' eqn: Heq'.
+revert s s' k k' l Heq Heq' Heqo.
+induction Hstep as
+ [ s A a f | s A B p f g | s A p1 p2 k | s A p1 p2 k |
+   s p k | s n p k | fuel s c p k Htrue | fuel s c p k Hfalse | s c p k |
+   s f | s s' f | s t f ];
+ intros s1 s2 k1 k2 l [= Hs1 Hk1] [= Hs2 Hk2] Heqo.
+- subst s1 k1 s2 k2.
+  by rewrite /= runbind runret.
+- subst s1 k1 s2 k2.
+  cbn.
+  by rewrite bindA.
+- subst s1 s2 k1 k2.
+  reflexivity.
+- subst s1 s2 k1 k2.
+  reflexivity.
+- subst.
+  cbn.
+  rewrite bindretf.
+  reflexivity.
+- subst.
+  cbn.
+  rewrite bindA.
+  reflexivity.
+- subst.
+  cbn.
+  rewrite bindA runbind runstget Htrue bindA.
+  reflexivity.
+- subst.
+  cbn.
+  rewrite bindA runbind runstget Hfalse bindretf.
+  reflexivity.
+- subst.
+  cbn.
+  rewrite bindretf.
+  reflexivity.
+- subst s1 k1 s2 k2.
+  by rewrite /= runbind runstget.
+- subst s1 k1 s2 k2.
+  by rewrite /= runbind runstput.
+- discriminate Heqo.
+Qed.
+
+Lemma step_Some_correct s s' k k' t l :
+  step (s, k) (Some t) (s', k') ->
+  Run (denote_continuation M k) (s, l) =
+  Run (denote_continuation M k') (s', rcons l t).
+Proof.
+intro Hstep.
+remember (s, k) as sk eqn: Heq.
+remember (Some t) as o eqn: Heqo.
+remember (s', k') as sk' eqn: Heq'.
+revert s s' k k' l Heq Heq' Heqo.
+induction Hstep as
+ [ s A a f | s A B p f g | s A p1 p2 k | s A p1 p2 k |
+   s p k | s n p k | fuel s c p k Htrue | fuel s c p k Hfalse | s c p k |
+   s f | s s' f | s t' f ];
+ intros s1 s2 k1 k2 l [= Hs1 Hk1] [= Hs2 Hk2] Heqo; try discriminate Heqo.
+subst s1 k1 s2 k2.
+injection Heqo; intro; subst t.
+by rewrite /= runbind runstmark.
+Qed.
+
+Lemma step_star_correct_gen s s' k k' l l' :
+  step_star (s, k) l' (s', k') ->
+  Run (denote_continuation M k) (s, l) = Run (denote_continuation M k') (s', l++l').
+Proof.
+intro Hstep_star.
+remember (s, k) as sk eqn: Heq.
+remember (s', k') as sk' eqn: Heq'.
+revert s s' k k' l Heq Heq'.
+induction Hstep_star as
+ [ s |
+  (s, k) (s', k') (s'', k'') l' Hstep Hstep_star IH |
+  (s, k) (s', k') (s'', k'') t l' Hstep Hstep_star IH ];
+ intros s1 s2 k1 k2 l1 Heq1 Heq2.
+- rewrite cats0.
+  by move: Heq2; rewrite Heq1 => -[<- <-].
+- move: Heq1 Heq2 => [<- <-] [<- <-].
+  apply step_None_correct with (l := l1) in Hstep.
+  rewrite Hstep.
+  apply IH; reflexivity.
+- move: Heq1 Heq2 => [<- <-] [<- <-].
+  apply step_Some_correct with (l := []) in Hstep.
+  rewrite <- cats0 at 1.
+  rewrite denote_continuation_prefix_independent; [ | now exists k ].
+  rewrite -> Hstep, (IH _ s'' _ k'');
+   [ | reflexivity | reflexivity ].
+  cbn.
+  rewrite denote_continuation_prefix_independent; [ reflexivity | ].
+  now eexists.
+Qed.
+
+Proposition step_star_correct
+  (s s' : S) (A : Type) (a : A) (p : program A) (l : list T) :
+  step_star (s, p `; stop A) l (s', stop A a) ->
+  Run (denote M _ p) (s, []) = (a, (s', l)).
+Proof.
+intro Hss.
+apply step_star_correct_gen with (l := []) in Hss.
+move: Hss.
+rewrite /= runret runbind.
+destruct (Run (denote M _ p) (s, [])) as [a'' [s'' l'']].
+rewrite runret => -[Heq3 <- <-].
+apply inj_pair2 in Heq3.
+by rewrite Heq3.
+Qed.
+
+Lemma step_star_complete_gen
+  (s s' : S) (A : Type) (a : A) (p : program A) (l1 l2 : list T) f :
+  Run (denote M _ p) (s, l1) = (a, (s', l1 ++ l2)) ->
+  step_star (s, p `; f) l2 (s', f a).
+Proof.
+revert s s' a l1 l2 f.
+induction p as [ A a | A B p IHp g IHg | A b p1 IHp1 p2 IHp2 |
+  n p IHp | fuel c p IHp | | s0' | t ]; cbn;
+ intros s s' a' l1 l2 f Heq.
+- rewrite runret in Heq.
+  injection Heq; clear Heq; intros; subst a' s'.
+  replace l2 with (@nil T) by
+   (revert l2 H; induction l1; [ tauto | intros ? [=]; firstorder ]).
+  eapply ss_step_None; [ apply s_ret | apply ss_refl ].
+- eapply ss_step_None.
+  + apply s_bind.
+  + move: Heq.
+    rewrite runbind.
+    case_eq (Run (denote M _ p) (s, l1)).
+    intros a (s0, l0) Hp Heq.
+    move: (denote_prefix_preserved ltac:(now eexists) Hp) => [l3 Hl3].
+    rewrite Hl3 in Hp.
+    apply IHp with (f := (fun a => g a `; f)) in Hp.
+    clear IHp.
+    move: (denote_prefix_preserved ltac:(now eexists) Heq) => [l4 Hl4].
+    rewrite Hl4 in Heq.
+    apply IHg with (f := f) in Heq.
+    clear IHg.
+    subst l0.
+    replace l2 with (l3 ++ l4) by
+     (induction l1; cbn in Hl4; [ congruence | injection Hl4; tauto ]).
+    eapply step_star_transitive.
+    * exact Hp.
+    * exact Heq.
+- destruct b; [
+    eapply ss_step_None; [
+      apply s_cond_true
+    | apply IHp1 with (l1 := l1); exact Heq ]
+  | eapply ss_step_None; [
+      apply s_cond_false
+    | apply IHp2 with (l1 := l1); exact Heq ]
+  ].
+- revert s l1 l2 Heq.
+  induction n as [ | n' IHn ]; intros s l1 l2 Heq.
+  + rewrite runret in Heq.
+    injection Heq; clear Heq; intros; subst a' s'.
+    replace l2 with (@nil T) by
+     (revert l2 H; induction l1; [ tauto | intros ? [=]; firstorder ]).
+    eapply ss_step_None; [ apply s_repeat_O | apply ss_refl ].
+  + rewrite runbind in Heq.
+    case_eq (Run (denote M _ p) (s, l1)).
+    intros a (s0, l0) Hp.
+    rewrite Hp in Heq.
+    move: (denote_prefix_preserved ltac:(now eexists) Hp) => [l3 Hl3].
+    rewrite Hl3 {l0 Hl3} in Hp, Heq.
+    specialize (IHp _ _ _ _ _ (fun _ => p_repeat n' p `; f) Hp).
+    assert (Heq':
+     Run (denote M _ (p_repeat n' p)) (s0, l1 ++ l3) = (a', (s', l1 ++ l2)))
+     by apply Heq.
+    move: (denote_prefix_preserved ltac:(now eexists) Heq') => [l4 Hl4].
+    rewrite Hl4 in Heq.
+    eapply ss_step_None; [ apply s_repeat_S | ].
+    have -> : l2 = l3 ++ l4.
+      by move/(congr1 (drop (size l1))) : Hl4; rewrite -catA ?drop_size_cat.
+    eapply step_star_transitive; [ eexact IHp | eapply IHn; eexact Heq ].
+- revert s l1 l2 Heq.
+  induction fuel as [ | fuel' IHn ]; intros s l1 l2 Heq.
+  + rewrite runret in Heq.
+    injection Heq; clear Heq; intros; subst a' s'.
+    replace l2 with (@nil T) by
+     (revert l2 H; induction l1; [ tauto | intros ? [=]; firstorder ]).
+    eapply ss_step_None; [ apply s_while_broke | apply ss_refl ].
+  + rewrite runbind runstget in Heq.
+    cbn in Heq.
+    case_eq (c s); [ intro Htrue | intro Hfalse ].
+    * rewrite Htrue runbind in Heq.
+      case_eq (Run (denote M _ p) (s, l1)).
+      intros a (s0, l0) Hp.
+      rewrite Hp in Heq.
+      move: (denote_prefix_preserved ltac:(now eexists) Hp) => [l3 Hl3].
+      rewrite Hl3 {l0 Hl3} in Hp, Heq.
+      specialize (IHp _ _ _ _ _ (fun _ => p_while fuel' c p `; f) Hp).
+      assert (Heq':
+       Run (denote M _ (p_while fuel' c p)) (s0, l1 ++ l3) = (a', (s', l1 ++ l2)))
+       by apply Heq.
+      move: (denote_prefix_preserved ltac:(now eexists) Heq') => [l4 Hl4].
+      rewrite Hl4 in Heq.
+      eapply ss_step_None; [ apply s_while_true; exact Htrue | ].
+      have -> : l2 = l3 ++ l4.
+        by move/(congr1 (drop (size l1))) : Hl4; rewrite -catA ?drop_size_cat.
+      eapply step_star_transitive; [ eexact IHp | eapply IHn; eexact Heq ].
+    * move: Heq; rewrite Hfalse runret.
+      move=> [<- <-] /(congr1 (drop (size l1))).
+      rewrite drop_size_cat // drop_size => <-.
+      eapply ss_step_None; [ apply s_while_false; exact Hfalse | apply ss_refl ].
+- move: Heq; rewrite runstget.
+  move=> [<- <-] /(congr1 (drop (size l1))).
+  rewrite drop_size_cat // drop_size => <-.
+  eapply ss_step_None; [ apply s_get | apply ss_refl ].
+- move: Heq; rewrite runstput.
+  move=> [<- <-] /(congr1 (drop (size l1))).
+  rewrite drop_size_cat // drop_size => <-.
+  eapply ss_step_None; [ apply s_put | apply ss_refl ].
+- move: Heq; rewrite runstmark.
+  move=> [<- <-] /(congr1 (drop (size l1))).
+  rewrite drop_size_cat // drop_rcons // drop_size => <-.
+  eapply ss_step_Some; [ apply s_mark | apply ss_refl ].
+Qed.
+
+Proposition step_star_complete
+  (s s' : S) (A : Type) (a : A) (p : program A) (l : list T) :
+  Run (denote M _ p) (s, []) = (a, (s', l)) ->
+  step_star (s, p `; stop A) l (s', stop A a).
+Proof.
+intro Hp.
+apply step_star_complete_gen with (l1 := []).
+exact Hp.
+Qed.
+
+End semantics_equivalence.
+
+Notation "'eT' x y" := (@existT _ _ x y) (at level 200).
+Notation "'e' x" := (@exist _ _ x _) (at level 200).
+
+Definition p_nonce : program nat :=
+  p_do n <- p_get;
+  p_do _ <- p_put (S n);
+  p_do _ <- p_mark n;
+  p_ret n.
+
+Definition M := @ModelStateTraceRun.mk.
+
+Eval unfold denote, p_nonce in denote (M nat nat) nat p_nonce.
+
+Local Open Scope do_notation.
+
+Definition nonce : M nat nat nat :=
+  do n : nat <- stGet;
+  do _ : unit <- stPut (S n);
+  do _ : unit <- stMark n;
+  Ret n.
+
+Compute nonce (0, []).
+Compute (denote (M nat nat) nat p_nonce) (0, []).
+Compute run_ss p_nonce 0.
+
+Remark denote_p_nonce : denote (M nat nat) nat p_nonce = nonce.
+Proof. by []. Qed.
+
+Program Example p_nonce_twice : program bool_eqType :=
+  p_do nonce <- p_ret (
+    p_do n : nat <- p_get;
+    p_do _ : unit <- p_put (S n);
+    p_do _ : unit <- p_mark n;
+    p_ret n ) ;
+  p_do x <- nonce ;
+  p_do y <- nonce ;
+  p_ret (x == y).
+
+Example nonce_twice : M _ _ _ :=
+  do nonce <- Ret (
+    do n : nat <- stGet;
+    do _ : unit <- stPut (S n);
+    do _ : unit <- stMark n;
+    Ret n ) ;
+  do x <- nonce ;
+  do y <- nonce ;
+  Ret (Nat.eqb x y).
+
+Compute nonce_twice (0, []).
+Compute (denote (M nat nat) bool p_nonce_twice) (0, []).
+Compute run_ss p_nonce_twice 0.
+
+Remark denote_p_nonce_twice :
+  denote (M nat nat) bool p_nonce_twice = nonce_twice.
+Proof. by []. Qed.
+
+Fixpoint countdown (fuel : nat) : M nat bool unit :=
+  match fuel with
+  | O => Ret tt
+  | S fuel' =>
+    do n <- stGet ;
+    if (n == 0) then
+      stMark true
+    else
+      do _ <- stMark false ; do _ <- stPut (n-1) ; countdown fuel'
+  end.
+
+Fixpoint p_countdown (fuel : nat) : program unit :=
+  match fuel with
+  | O => p_ret tt
+  | S fuel' =>
+    p_do n <- p_get ;
+    p_cond (n == 0) (
+      p_mark true
+    ) (
+      p_do _ <- p_mark false ; p_do _ <- p_put (n-1) ; p_countdown fuel'
+    )
+  end.
+
+Compute (countdown 100) (5, []).
+Compute (denote (M nat bool) unit (p_countdown 100)) (5, []).
+Compute run_ss (p_countdown 100) 5.
+
+Remark denote_countdown fuel :
+  denote (M nat bool) unit (p_countdown fuel) = countdown fuel.
+Proof.
+elim: fuel => // n.
+rewrite [countdown (S n)]/=.
+by move <-.
+Qed.
+
+Example p_multiply (a b : nat) : program (T := unit) unit :=
+  p_do _ <- p_put 0 ;
+  p_repeat b (
+    p_do x <- p_get ;
+    p_put (a + x)
+  ).
+
+Compute run_ss (p_multiply 3 7) 0.
+
+Example p_division (a b : nat) : program (T := unit) unit :=
+  p_do _ <- p_put (a, 0);
+  p_while a (fun s => b <= fst s) (
+    p_do s <- p_get ;
+    p_put (fst s - b, S (snd s))
+  ).
+
+Compute run_ss (p_division 22 7) (0, 0).
+
+Compute run_s_n 15 (p_division 22 7) (stop unit) (0, 0).
