impredicative_set/iparametricity.v
@@ -1,10 +1,9 @@
 Declare ML Module "paramcoq".
 
 From mathcomp Require Import all_ssreflect.
-Require Import hierarchy monad mmt_sect5 monad_model.
-Import Univ.
+Require Import ihierarchy imonad immt_sect5 imonad_model.
 
-Unset Universe Checking.
+Import Univ.
 Set Bullet Behavior "Strict Subproofs".
 
 (** The identity monad *)
@@ -12,17 +11,17 @@ Module Identity.
 
 Section Naturality.
 
-Variable A : UU1.
+Variable A : UU0.
 
 Realizer A as A_R := (@eq A).
 
-Definition M (X : UU1) : UU1 :=
+Definition M (X : UU0) : UU0 :=
 ltac:(
   let t := constr:(ModelMonad.identity X) in
   let t := eval cbn in t in
   exact t).
 
-Definition T : UU1 := k_type M A.
+Definition T : UU0 := k_type M A.
 
 Parametricity T arity 2.
 
@@ -53,18 +52,18 @@ Module Exception.
 
 Section Naturality.
 
-Variables E A : UU1.
+Variables E A : UU0.
 
 Realizer E as E_R := (@eq E).
 Realizer A as A_R := (@eq A).
 
-Definition M (X : UU1) : UU1 := 
+Definition M (X : UU0) : UU0 := 
 ltac:(
   let t := constr:(ModelMonad.Except.t E X) in
   let t := eval cbn in t in
   exact t).
 
-Definition T : UU1 := k_type M A.
+Definition T : UU0 := k_type M A.
 
 Parametricity Recursive T arity 2.
 
@@ -104,11 +103,11 @@ Module Option.
 
 Section Naturality.
 
-Variable A : UU1.
+Variable A : UU0.
 
-Definition M (X : UU1) : UU1 := ModelMonad.option_monad X.
+Definition M (X : UU0) : UU0 := ModelMonad.option_monad X.
 
-Definition T : UU1 := k_type M A.
+Definition T : UU0 := k_type M A.
 
 Variable m : T.
 
@@ -128,17 +127,17 @@ Module List.
 
 Section Naturality.
 
-Variable A : UU1.
+Variable A : UU0.
 
 Realizer A as A_R := (@eq A).
 
-Definition M (X : UU1) : UU1 :=
+Definition M (X : UU0) : UU0 :=
 ltac:(
   let t := constr:(ModelMonad.ListMonad.t X) in
   let t := eval cbn in t in
   exact t).
 
-Definition T : UU1 := k_type M A.
+Definition T : UU0 := k_type M A.
 
 Parametricity Recursive T arity 2.
 
@@ -189,18 +188,18 @@ Module State.
 
 Section Naturality.
 
-Variable S A : Type.
+Variable S A : UU0.
 
 Realizer S as S_R := (@eq S).
 Realizer A as A_R := (@eq A).
 
-Definition M X : Type :=
+Definition M X : UU0 :=
 ltac:(
   let t := constr:(ModelMonad.State.t S X) in
   let t := eval cbn in t in
   exact t).
 
-Definition T : UU1 := k_type M A.
+Definition T : UU0 := k_type M A.
 
 Parametricity Recursive T arity 2.
 
